$$
F(x)*G(x) - 1 \equiv 0 \mod x^n
$$

$$
G_t(x) * F(x) - 1 \equiv 0\mod x^{2^t}
$$

$$
G_{t+1}(x) * F(x) - 1 \equiv 0\mod x^{2^{t+1}}
$$

$$
0 \equiv G_{t}(x)F(x) -1 + F(x)*(G_{t+1}(x) - G_t(x))\mod x^{2^{t+1}}
$$

$$
0 \equiv G_t(x)*G_t(x)*F(x) - G_t(x) + G_{t+1}(x) - G_{t}(x)\mod x^{2^{t+1}}
$$

$$
G_{t+1}(x) \equiv -G_t(x)*G_t(x)*F(x) + 2*G_t(x)
$$

$$
ln(f(x)) = g(x)\mod x^n
$$

$$
只需\frac {f'(x)} {f(x)} = g'(x)\mod x^{n-1}
$$

$$
所以g(x) = \int\frac{f'(x)}{f(x)}dx \mod x^n
$$

$$
G(x) \equiv exp(F(x))\mod x^n
$$

$$
ln(G(x)) - F(x)\equiv 0\mod x^n
$$

$$
[x^0]G(x) = 1
$$

$$
G_{t+1}(x) \equiv G_t(x) - G_t(x)ln(G_t(x)) + G_t(x)F(x)\mod x^{2^{t+1}}
$$

$$
欧拉定理：
若(a,p) =1,则a^{m} \equiv a^{m \%phi(p)}\mod p
$$

